theories/zoo_kcas/kcas_2.v
@@ -1,0 +1,12 @@
+From zoo Require Import
+  prelude.
+From zoo_kcas Require Import
+  kcas_2__types.
+From zoo_kcas Require Export
+  kcas_2__code.
+From zoo Require Import
+  options.
+
+#[global] Opaque kcas_2_make.
+#[global] Opaque kcas_2_get.
+#[global] Opaque kcas_2_cas.
